src_arrays/Dijkstra_generic.v
@@ -12,6 +12,8 @@ Require Import Lia.
 Require Import src_arrays.Tactics.
 Require Import src_arrays.Interweave.
 
+Require Import graphs.Graphs.
+
 Definition init_array : Value string :=
   [-\] "array", [-\] "size", [-\] "value",
     [let "i"] Ref (Int 0) [in]
@@ -46,7 +48,7 @@ Definition generic_dijkstra (get_size get_neighbours mkheap h_insert h_empty h_e
         [let "rec_current"] h_extract_min <* (Var "h") [in]
         [let "current"] Get 0 (Var "rec_current") [in]
         [let "dist_current"] Get 1 (Var "rec_current") [in]
-        [let "neighs"] Ref (get_neighbours <* Var "current") [in]
+        [let "neighs"] Ref (get_neighbours <* Var "g" <* Var "current") [in]
         (* neighs : a reference to a list *)
           [while] [~] (l_is_nil <* Var "neighs") [do]
             [let "rec_neigh"] l_head <* Var "neighs" [in]
@@ -71,14 +73,15 @@ Definition generic_dijkstra (get_size get_neighbours mkheap h_insert h_empty h_e
             [end]
             [end];;
             Var "neighs" <- l_tail <* Var "neighs"
-          [end]
+          [end];;
+          Free (Var "neighs")
         [end]
         [end]
         [end]
         [end]
       [end];;
       h_free <* (Var "h");;
-      Var "dist"
+      RecV [Var "dist"; Var "pred"]
       (*
       [let "x"] ! (Var "dist" >> Var "dst") [in]
         free_array <* (Var "dist");;
@@ -91,21 +94,148 @@ Definition generic_dijkstra (get_size get_neighbours mkheap h_insert h_empty h_e
     [end]
     [end]%string.
 
-Parameter is_graph : forall {V}, Label -> StateAssertion V.
-Parameter dists_in_graph : forall {V}, Label -> Label -> StateAssertion V.
-Parameter in_graph : forall {V}, Label -> Label -> StateAssertion V.
-Parameter dist_in_graph : forall {V}, Label -> Z -> Z -> nat -> StateAssertion V.
+Definition is_elem_list {A} (P : A -> Prop) (L : list A) :=
+  forall x, List.In x L <-> P x.
 
-Parameter get_size get_neighbours mkheap h_insert h_empty h_extract_min h_decrease_key h_free l_is_nil l_head l_tail : Value string.
+Definition is_elem_weighted_list {A B} (P : A -> Prop) (W : A -> B) (L : list (A * B)) :=
+  forall x w, List.In (x,w) L <-> (P x /\ w = W x).
 
-Theorem triple_fun_generic_dijkstra l src dst :
+Definition is_elem_unique_list {A} (P : A -> Prop) (L : list A) :=
+  is_elem_list P L /\ List.NoDup L.
+
+Definition is_elem_weighted_unique_list {A B} (P : A -> Prop) (W : A -> B) (L : list (A * B)) :=
+  is_elem_weighted_list P W L /\ List.NoDup L.
+
+Definition is_set_size {A} (P : A -> Prop) (n : nat) : Prop :=
+  exists l, is_elem_unique_list P l /\ List.length l = n.
+
+Parameter is_list : forall {V}, list (Value V) -> Value V -> StateAssertion V.
+
+Definition nat2value {V} (n : nat) : Value V := Int (Z.of_nat n).
+Definition pair2Value {A B V} (f : A -> Value V) (g : B -> Value V) '(x,y) : Value V :=
+  RecV [f x; g y].
+
+Definition nats2values {V} (L : list nat) : list (Value V) :=
+  List.map (fun t => Int (Z.of_nat t)) L.
+Definition nat_pairs2values {V} (L : list (nat * nat)) : list (Value V) :=
+  List.map (fun '(x,w) => RecV [Int (Z.of_nat x); Int (Z.of_nat w)]) L.
+
+Inductive is_graph {A} : graph nat -> Value A -> StateAssertion A :=
+| is_graph_intro n g c m :
+  (forall i, V g i ->
+    exists v Lv L,
+      Lookup (OfNat (n + i)) m v /\
+      is_list Lv v c m /\
+      is_elem_unique_list (neighbours g i) L /\
+      Lv = nats2values L) ->
+  is_graph g (Lab (OfNat n)) c m.
+
+Inductive is_weighted_graph {A} : wgraph nat -> Value A -> StateAssertion A :=
+| is_weighted_graph_intro n (g : wgraph nat) c m :
+  (forall i, V g i ->
+    exists v Lv L,
+      Lookup (OfNat (n + i)) m v /\
+      is_list Lv v c m /\
+      is_elem_weighted_unique_list (neighbours g i) (W g i) L /\
+      Lv = nat_pairs2values L) ->
+  is_weighted_graph g (Lab (OfNat n)) c m.
+
+Definition is_nat_function {V} (f : nat -> option nat) '(OfNat n0) : StateAssertion V :=
+  fun c m =>
+    forall n n', f n = Some n' <-> Lookup (OfNat (n0+n)) m (Int (Z.of_nat n')).
+
+(*Parameter get_size get_neighbours mkheap h_insert h_empty h_extract_min h_decrease_key h_free l_is_nil l_head l_tail : Value string.*)
+
+Definition get_size_spec {A} g (get_size : Value A) : Prop :=
+  triple_fun get_size
+    (is_weighted_graph g)
+    (fun v => <exists> n v', <[v = Int (Z.of_nat n)]> <*> <[is_set_size (V g) n]> <*> is_weighted_graph g v').
+
+Definition get_neighbours_spec {A} l n (g : wgraph nat) (get_neighbours : Value A) : Prop :=
+  triple_fun get_neighbours
+    (fun v => <[v = Lab l]>)
+    (fun v => <[
+      triple_fun v
+        (fun v => <[v = Int (Z.of_nat n)]> <*> <[V g n]> <*> is_weighted_graph g (Lab l))
+        (fun v => <exists> L, <[is_elem_weighted_unique_list (neighbours g n) (W g n) L]> <*> is_list (nat_pairs2values L) v </\> is_weighted_graph g (Lab l))
+    ]>).
+
+Parameter is_heap : forall {V} (n : nat) (P : nat -> Prop) (W : nat -> option nat), Value V -> StateAssertion V.
+
+Definition mkheap_spec {V} n (mkheap : Value V) : Prop :=
+  triple_fun mkheap
+    (fun v => <[v = Int (Z.of_nat n)]>)
+    (is_heap n empty (fun _ => None)).
+
+Definition set_value_at (W : nat -> option nat) (x y n : nat) : option nat :=
+  if n =? x then Some y else W n.
+
+Definition h_insert_spec {V}
+  n (P : nat -> Prop) (W : nat -> option nat) h (s k d : nat) (h_insert : Value V) : Prop :=
+  is_set_size P s ->
+  s < n ->
+  ~ P k ->
+  triple_fun h_insert
+    (fun v => <[v = h]>)
+    (fun v => <[
+      triple_fun v
+        (fun v => <[v = Int (Z.of_nat k)]>)
+        (fun v => <[
+          triple_fun v
+            (fun v => <[v = Int (Z.of_nat d)]> <*> is_heap n P W h)
+            (fun v => <[v = U_val]> <*> is_heap n (set_sum P (single k)) (set_value_at W k d) h)
+        ]>)
+    ]>).
+
+Definition h_empty_spec {V} n (P : nat -> Prop) (W : nat -> option nat) h s (h_empty : Value V) : Prop :=
+  is_set_size P s ->
+  triple_fun h_empty
+    (fun v => <[v = h]> <*> is_heap n P W h)
+    (fun v => <[v = Bool (s =? 0)]> <*> is_heap n P W h).
+
+Definition unset_value_at (W : nat -> option nat) (x n : nat) : option nat :=
+  if n =? x then None else W n.
+
+Definition set_remove {A} (P : A -> Prop) (x y : A) : Prop :=
+  P y /\ y <> x.
+
+Definition h_extract_min_spec {V}
+  n (P : nat -> Prop) (W : nat -> option nat) h k d (h_extract_min : Value V) : Prop :=
+  min_cost_elem P W k ->
+  W k = Some d ->
+  triple_fun h_extract_min
+    (fun v => <[v = h]> <*> is_heap n P W h)
+    (fun v => <[v = pair2Value nat2value nat2value (k,d)]> <*> is_heap n (set_remove P k) W h).
+
+Definition h_decrease_key_spec {V}
+  n (P : nat -> Prop) (W : nat -> option nat) h k d (h_decrease_key : Value V) : Prop :=
+  P k ->
+  triple_fun h_decrease_key
+    (fun v => <[v = h]>)
+    (fun v => <[
+      triple_fun v
+        (fun v => <[v = Int (Z.of_nat k)]>)
+        (fun v => <[
+          triple_fun v
+            (fun v => <[v = Int (Z.of_nat d)]> <*> is_heap n P W h)
+            (fun v => <[v = U_val]> <*> is_heap n P (set_value_at W k d) h)
+        ]>)
+    ]>).
+
+Definition h_free_spec {V}
+  n (P : nat -> Prop) (W : nat -> option nat) (h_free : Value V) : Prop :=
+  triple_fun h_free
+    (is_heap n P W)
+    (fun v => <[]>).
+
+Theorem triple_fun_generic_dijkstra
+  (get_size get_neighbours mkheap h_insert h_empty h_extract_min h_decrease_key h_free l_is_nil l_head l_tail : Value string)
+  g l src D pred :
   triple_fun
     (generic_dijkstra get_size get_neighbours mkheap h_insert h_empty h_extract_min h_decrease_key h_free l_is_nil l_head l_tail)
     (fun v => <[v = Lab l]>)
     (fun v => <[triple_fun v
-      (fun v => <[v = Int src]>)
-      (fun v => <[triple_fun v
-        (fun v => <[v = Int dst]> <*> is_graph l)
-        (fun v => <exists> n, <[v = Int (Z.of_nat n)]> <*> is_graph l <*> dist_in_graph l src dst n)]>)]>).
+      (fun v => <[v = Int (Z.of_nat src)]> <*> is_weighted_graph g (Lab l) <*> <[V g src]> <*> <[Dijkstra_initial D pred src]>)
+        (fun v => <exists> lD lpred, <[v = RecV [Lab lD; Lab lpred]]> <*> is_weighted_graph g (Lab l) <*> is_nat_function D lD <*> is_nat_function pred lpred <*> <[Dijkstra_final D pred src g]>)]>).
 Proof.
 Admitted.
